Examples.lean
@@ -10,6 +10,7 @@ import Examples.Language.Remainder
 import Examples.Language.Scalar
 import Examples.Language.ScalarCompiled
 import Examples.Language.Traversal
+import Examples.Language.TraversalCompiled
 import Examples.Ram.AmortizedClear
 import Examples.Ram.Arithmetic
 import Examples.Ram.ArrayArguments
